new/golang/defn/builtin.v
@@ -23,5 +23,6 @@ Axiom int_lt : val.
 Axiom int_leq : val.
 Axiom int_geq : val.
 Axiom int_gt : val.
+Axiom int_quot : val.
 
 End goose_lang.
